# explaination

given the transformation

  ```math?:
  T:
    a <- a+b
    b <- a
  ```

and the transformation

  ```math?:
  Tpq:
    a <- bq + aq + ap
    b <- bp + aq
  ```

If we see that the transformation T is actually the transformation Tpq with p = 0 and
q = 1, we can prove that applying t T (so Tpq with p = 0 and q = 1) twice is the same
as applying a transformation Tp'q' once, where p' = q and q' = p + q

I got to this answer by working through 5 applications of T and bringing the result
back in line with Tpq; i am not sure how applying T twice is the same as squaring, but
it was not a goal of the exercise.

---

checked a solution and this is wrong, i don't have to apply T twice, but Tpq...
what went wrong here: i didn't understand what i had to do from the exercise text.
